update

03_Fixpoint_Earley_Recognizer.thy
@@ -2,7 +2,6 @@
 theory "03_Fixpoint_Earley_Recognizer"
   imports
     "02_Earleys_Algorithm"
-    "HOL-Library.LaTeXsugar"
 begin
 (*>*)
 
@@ -40,7 +39,7 @@ projections accessing the specific part of the instance @{term cfg} of the datat
 and a right-hand side or @{term rule_body}, a list of symbols.
 The productions with a particular nonterminal $N$ on their left-hand sides are called the alternatives of $N$.
 We make the usual assumptions about the well-formedness of a context-free grammar: the intersection of the set of terminals and
-the set of nonterminals is empty; the start symbol @{term \<SS>} is a nonterminal; the rule head of a production
+the set of nonterminals is empty; the start symbol is a nonterminal; the rule head of a production
 is a nonterminal and its rule body consists of only symbols. Additionally, since we are working with
 a list of productions, we make the assumption that this list is distinct.
 \<close>
@@ -84,10 +83,10 @@ inductively using the keyword \textit{inductive\_set}.
 
 Next we formalize the concept of a derivation. We use lowercase letters $a$, $b$, $c$ indicating terminal symbols; capital letters
 $A$, $B$, $C$ denote nonterminals; lists of symbols are represented by greek letters: \alpha, \beta, \gamma, occasionally also by lowercase letters $u$, $v$, $w$.
-The empty list in the context of a language is \epsilon. A sentential is a list $\alpha$ consisting of only symbols. A sentence
-is a sentential if it only contains terminal symbols. We first define a predicate \textit{derives1} which expresses that
-we can derive $v$ from $u$ in a single step or @{term "derives1 cfg u v"} holds if there exist $\alpha$, $\beta$, $N$ and $\gamma$ such that @{term "u = \<alpha> @ [N] @ \<beta>"},
-@{term "v = \<alpha> @ \<gamma> @ \<beta>"} and @{term "(N, \<gamma>)"} is a production rule. We then can define the set of single-step derivations,
+The empty list in the context of a language is \epsilon. A sentential is a list consisting of only symbols. A sentence
+is a sentential if it only contains terminal symbols. We first define a predicate @{term "derives1 cfg u v"} which expresses that
+we can derive $v$ from $u$ in a single step or the predicate holds if there exist $\alpha$, $\beta$, $N$ and $\gamma$ such that @{term "u = \<alpha> @ [N] @ \<beta>"},
+@{term "v = \<alpha> @ \<gamma> @ \<beta>"} and @{term "(N, \<gamma>)"} is a production rule. We then can define the set of single-step derivations using @{term derives1},
 and subsequently the set of all derivations given a particular grammar is the reflexive-transitive closure of the set of
 single-step derivations. Finally, we say $v$ can be derived from $u$ given a grammar \textit{cfg}, or @{term "derives cfg u v"} if
 @{term "(u, v) \<in> derivations cfg"}.
@@ -128,7 +127,7 @@ definition derives :: "'a cfg \<Rightarrow> 'a sentential \<Rightarrow> 'a sente
 
 text\<open>
 Potentially recursive but provably total functions that may make use of pattern matching are defined with
-the \textit{fun} and \textit{function} keywords; partial functions are defined via \textit{partial\_function}
+the \textit{fun} and \textit{function} keywords; partial functions are defined via \textit{partial\_function}.
 Take for example the function @{term slice} defined below. Term @{term "slice i j xs"} computes the slice of a list @{term xs}
 between indices $i$ (inclusive) and $j$ (exclusive), e.g. @{term "slice (2::nat) (4::nat) [a, b, c, d, e]"} evaluates to @{term "[c, d]"}.
 \<close>
@@ -156,7 +155,7 @@ lemma slice_append:
 section \<open>Earley's Algorithm \label{sec:earley}\<close>
 
 text\<open>
-Now we are ready to formalize the algorithm presented in Chapter \ref{chapter:2}. First we define the datatype @{term item}
+Next we formalize the algorithm presented in Chapter \ref{chapter:2}. First we define the datatype @{term item}
 representing Earley items. For example, the item $S \rightarrow \, S + \bullet S, 2, 4$ consists of four parts:
 a production rule (@{term item_rule}), a natural number (@{term item_bullet}) indicating the position of the bullet in
 the production rule, and two natural numbers (@{term item_origin} inclusive, @{term item_end} exclusive) representing the portion
@@ -167,7 +166,7 @@ We call an item @{term complete} if the bullet is at the end of the production r
 an item is either @{term None} if it is complete, or @{term "Some s"} where $s$ is the symbol in the production
 rule body following the bullet. An item is finished if the item rule head is the start symbol, the item is complete, and
 the whole input has been scanned or @{term "item_origin item = (0::nat)"} and @{term "item_end item = length \<omega>"}. Finally, we call a set of
-items @{term recognizing} if it contains at least one finished item.
+items @{term recognizing} if it contains at least one finished item, indicating that this set of items recognizes the input $\omega$.
 \<close>
 
 datatype 'a item = 
@@ -198,14 +197,14 @@ definition next_symbol :: "'a item \<Rightarrow> 'a option" where
   "next_symbol x \<equiv> if is_complete x then None else Some ((item_rule_body x) ! (item_bullet x))"
 
 definition is_finished :: "'a cfg \<Rightarrow> 'a sentential \<Rightarrow> 'a item \<Rightarrow> bool" where
-  "is_finished cfg inp x \<equiv> 
+  "is_finished cfg \<omega> x \<equiv> 
     item_rule_head x = \<SS> cfg \<and>
     item_origin x = 0 \<and>
-    item_end x = length inp \<and> 
+    item_end x = length \<omega> \<and> 
     is_complete x"
 
 definition recognizing :: "'a items \<Rightarrow> 'a cfg \<Rightarrow> 'a sentential \<Rightarrow> bool" where
-  "recognizing I cfg inp \<equiv> \<exists>x \<in> I. is_finished cfg inp x"
+  "recognizing I cfg \<omega> \<equiv> \<exists>x \<in> I. is_finished cfg \<omega> x"
 
 text\<open>
 Normally we don't construct items directly via the @{term Item} constructor but use two auxiliary constructors:
@@ -224,20 +223,20 @@ definition inc_item :: "'a item \<Rightarrow> nat \<Rightarrow> 'a item" where
   "inc_item x k = Item (item_rule x) (item_bullet x + 1) (item_origin x) k"
 
 text\<open>
-There are different approaches of defining the set of Earley items in accordance the rules of Figure \ref{fig:inference_rules}.
+There are different approaches of defining the set of Earley items in accordance with the rules of Figure \ref{fig:inference_rules}.
 We can take an abstract approach and define the set inductively using Isabelle's inductive sets,
 or a more operational point of view. We take the latter approach and discuss the reasoning for this
 decision end the end of this section.
 
-Note that, even though we are only constructing one set of Earley items, conceptually all items with the same item end
+Note that, as mentioned previously, even though we are only constructing one set of Earley items, conceptually all items with the same item end
 form one Earley bin. Our operational approach is then the following: we generate Earley items bin by bin in ascending order,
-starting from the $0$-th bin which contains all initial items. The three operations @{term Scan}, @{term Predict}, and @{term Complete}
-all take as an arguments the index of the current bin and the current set of Earley items. For the $k$-th bin
+starting from the $0$-th bin which contains all initial items computed by the @{term Init} operation. The three operations @{term Scan}, @{term Predict}, and @{term Complete}
+all take as arguments the index of the current bin and the current set of Earley items. For the $k$-th bin
 the @{term Scan} operation initializes the $k+1$-th bin, whereas the @{term Predict} and @{term Complete} operations
 only generate items belonging to the $k$-th bin. We then define a function @{term E_step} (short for Earley step) that
 returns the union of applying the three operations to a set of Earley items and this set itself. We complete the $k$-th
 bin and initialize the $k+1$-th bin by iterating @{term E_step} until the set of items stabilizes, captured by the @{term E_bin}
-definition. The function @{term \<E>} generates the bins up to the $n$-th bin by applying the @{term E_bin}
+definition. The function @{term \<E>} then generates the bins up to the $n$-th bin by applying the @{term E_bin}
 function first to the initial set of items @{term Init} and continuing in ascending order bin by bin. Finally, we compute
 the set of Earley items by applying @{term \<E>} to the length of the input.
 \<close>
@@ -249,11 +248,11 @@ definition Init :: "'a cfg \<Rightarrow> 'a items" where
   "Init cfg = { init_item r 0 | r. r \<in> set (\<RR> cfg) \<and> fst r = (\<SS> cfg) }"
 
 definition Scan :: "nat \<Rightarrow> 'a sentential \<Rightarrow> 'a items \<Rightarrow> 'a items" where
-  "Scan k inp I = 
+  "Scan k \<omega> I = 
     { inc_item x (k+1) | x a.
         x \<in> bin I k \<and>
-        inp!k = a \<and>
-        k < length inp \<and>
+        \<omega>!k = a \<and>
+        k < length \<omega> \<and>
         next_symbol x = Some a }"
 
 definition Predict :: "nat \<Rightarrow> 'a cfg \<Rightarrow> 'a items \<Rightarrow> 'a items" where
@@ -272,7 +271,7 @@ definition Complete :: "nat \<Rightarrow> 'a items \<Rightarrow> 'a items" where
         next_symbol x = Some (item_rule_head y) }"
 
 definition E_step :: "nat \<Rightarrow> 'a cfg \<Rightarrow> 'a sentential \<Rightarrow> 'a items \<Rightarrow> 'a items" where
-  "E_step k cfg inp I = I \<union> Scan k inp I \<union> Complete k I \<union> Predict k cfg I"
+  "E_step k cfg \<omega> I = I \<union> Scan k \<omega> I \<union> Complete k I \<union> Predict k cfg I"
 
 fun funpower :: "('a \<Rightarrow> 'a) \<Rightarrow> nat \<Rightarrow> ('a \<Rightarrow> 'a)" where
   "funpower f 0 x = x"
@@ -285,195 +284,338 @@ definition limit :: "('a set \<Rightarrow> 'a set) \<Rightarrow> 'a set \<Righta
   "limit f x = natUnion (\<lambda> n. funpower f n x)"
 
 definition E_bin :: "nat \<Rightarrow> 'a cfg \<Rightarrow> 'a sentential \<Rightarrow> 'a items \<Rightarrow> 'a items" where
-  "E_bin k cfg inp I = limit (E_step k cfg inp) I"
+  "E_bin k cfg \<omega> I = limit (E_step k cfg \<omega>) I"
 
 fun \<E> :: "nat \<Rightarrow> 'a cfg \<Rightarrow> 'a sentential \<Rightarrow> 'a items" where
-  "\<E> 0 cfg inp = E_bin 0 cfg inp (Init cfg)"
-| "\<E> (Suc n) cfg inp = E_bin (Suc n) cfg inp (\<E> n cfg inp)"
+  "\<E> 0 cfg \<omega> = E_bin 0 cfg \<omega> (Init cfg)"
+| "\<E> (Suc n) cfg \<omega> = E_bin (Suc n) cfg \<omega> (\<E> n cfg \<omega>)"
 
 definition earley :: "'a cfg \<Rightarrow> 'a sentential \<Rightarrow> 'a items" where
-  "earley cfg inp = \<E> (length inp) cfg inp"
+  "earley cfg \<omega> = \<E> (length \<omega>) cfg \<omega>"
 
 text\<open>
-We followed this operational approach of defining the set of Earley items primarily for two reasons: first of all, we adapted
+We followed the operational approach of defining the set of Earley items primarily for two reasons: first of all, we adapted
 most of the definitions of this chapter from the work on Local Lexing \cite{Obua:2017} \cite{LocalLexing-AFP},
-which takes the more operational approach and already defines useful lemmas for example on function iteration.
+which takes the more operational approach and already defines useful lemmas, for example on function iteration.
 Secondly, the operational approach maps more easily to the list-based implementation of the next chapter which
-necessarily takes an ordered approach to generating Earley items. Nonetheless, in hindsight defining the set
-of Earley items seems to be not only the more elegant approach but also might simplify some of the proofs of
+necessarily takes an ordered approach to generating Earley items. Nonetheless, in hindsight, defining the set
+of Earley items inductively seems to be not only the more elegant approach but also might simplify some of the proofs of
 this chapter.
 \<close>
 
 section \<open>Well-formedness\<close>
 
 text\<open>
-TODO:
+Due to the operational view of generating the set of Earley items, the proofs of, not only, well-formedness, but
+also soundness and completeness follow the same structure: we first proof a property about the basic building
+blocks, the @{term Init}, @{term Scan}, @{term Predict}, and @{term Complete} operations. Then, we proof that
+this property is maintained iterating the function @{term E_step}, and thus holds for the @{term E_bin} operation.
+Finally, we show that the function @{term \<E>} maintains this property for all conceptual bins and thus for the @{term earley} definition, or
+the set of Earley items.
 
-We define what it means for an item to be well-formed (@{term wf_item}): the item rule must be
-in the rules of the grammar; the item bullet has to be bounded by the length of the item rule body; the
-item origin should not exceed the item end, and finally the item end is at most the length of the input.
+Before we start to proof soundness and completeness of the generated set of Earley items, especially the
+completeness proof is more involved, we highlight the general proof structure once in detail, for a simpler
+property: well-formedness of the items, allowing us to concentrate only on the core aspects for the soundness
+and completeness proofs.
+
+An Earley item is well-formed (@{term wf_item}) if the item rule is a rule of the grammar; the item
+bullet is bounded by the length of the item rule body; the item origin does not exceed the item end, and
+finally the item end is at most the length of the input.
 \<close>
 
 definition wf_item :: "'a cfg \<Rightarrow> 'a sentential => 'a item \<Rightarrow> bool" where 
-  "wf_item cfg inp x \<equiv> 
+  "wf_item cfg \<omega> x \<equiv> 
     item_rule x \<in> set (\<RR> cfg) \<and> 
     item_bullet x \<le> length (item_rule_body x) \<and>
     item_origin x \<le> item_end x \<and> 
-    item_end x \<le> length inp"
+    item_end x \<le> length \<omega>"
 
 definition wf_items :: "'a cfg \<Rightarrow> 'a sentential \<Rightarrow> 'a items \<Rightarrow> bool" where
-  "wf_items cfg inp I \<equiv> \<forall>x \<in> I. wf_item cfg inp x"
+  "wf_items cfg \<omega> I \<equiv> \<forall>x \<in> I. wf_item cfg \<omega> x"
 
 lemma wf_Init:
-  assumes "x \<in> Init cfg"
-  shows "wf_item cfg inp x"
+  shows "wf_items cfg \<omega> (Init cfg)"
 (*<*)
   sorry
 (*>*)
-text\<open>by definition\<close>
+
+text\<open>\<close>
 
 lemma wf_Scan_Predict_Complete:
-  assumes "wf_items cfg inp I" 
-  shows "wf_items cfg inp (Scan k inp I \<union> Predict k cfg I \<union> Complete k I)"
+  assumes "wf_items cfg \<omega> I" 
+  shows "wf_items cfg \<omega> (Scan k \<omega> I \<union> Predict k cfg I \<union> Complete k I)"
 (*<*)
   sorry
 (*>*)
-text\<open>by definition\<close>
+
+text\<open>\<close>
 
 lemma wf_E_step:
-  assumes "wf_items cfg inp I"
-  shows "wf_items cfg inp (E_step k cfg inp I)"
+  assumes "wf_items cfg \<omega> I"
+  shows "wf_items cfg \<omega> (E_step k cfg \<omega> I)"
 (*<*)
   sorry
 (*>*)
-text\<open>@{thm[source] wf_Scan_Predict_Complete} by definition\<close>
+
+text\<open>
+Lemmas @{thm[source] wf_Init}, @{thm[source] wf_Scan_Predict_Complete}, and @{thm[source] wf_E_step}
+follow trivially by definition of the respective operations.
+\<close>
 
 lemma wf_funpower:
-  assumes "wf_items cfg inp I"
-  shows " wf_items cfg inp (funpower (E_step k cfg inp) n I)"
+  assumes "wf_items cfg \<omega> I"
+  shows "wf_items cfg \<omega> (funpower (E_step k cfg \<omega>) n I)"
 (*<*)
   sorry
 (*>*)
-text\<open>@{thm[source] wf_E_step}, by induction on n\<close>
+
+text\<open>\<close>
 
 lemma wf_E_bin:
-  assumes "wf_items cfg inp I"
-  shows "wf_items cfg inp (E_bin k cfg inp I)"
+  assumes "wf_items cfg \<omega> I"
+  shows "wf_items cfg \<omega> (E_bin k cfg \<omega> I)"
 (*<*)
   sorry
 (*>*)
-text\<open>@{thm[source] wf_funpower} by definition\<close>
+
+text\<open>\<close>
 
 lemma wf_E_bin0:
-  shows "wf_items cfg inp (E_bin 0 cfg inp (Init cfg))"
+  shows "wf_items cfg \<omega> (E_bin 0 cfg \<omega> (Init cfg))"
 (*<*)
   sorry
 (*>*)
-text\<open>@{thm[source] wf_Init} @{term wf_E} by definition\<close>
+
+text\<open>
+We proof the lemma @{thm[source] wf_funpower} by induction on $n$ using @{thm[source] wf_E_step}, and
+lemmas @{thm[source] wf_E_bin} and @{thm[source] wf_E_bin0} follow immediately using additionally the fact
+that @{term "x \<in> limit f X \<equiv> \<exists>n. x \<in> funpower f n X"} and lemma @{thm[source] wf_Init}.
+\<close>
 
 lemma wf_\<E>:
-  shows "wf_items cfg inp (\<E> n cfg inp)"
+  shows "wf_items cfg \<omega> (\<E> n cfg \<omega>)"
 (*<*)
   sorry
 (*>*)
-text\<open>@{thm[source] wf_E_bin0} @{thm[source] wf_E_bin} by induction on n\<close>
+
+text\<open>\<close>
 
 lemma wf_earley:
-  shows "wf_items cfg inp (earley cfg inp)"
+  shows "wf_items cfg \<omega> (earley cfg \<omega>)"
 (*<*)
   sorry
 (*>*)
-text\<open>@{thm[source] wf_\<E>} by definition\<close>
+
+text\<open>
+Finally, lemma @{thm[source] wf_\<E>} is proved by induction on $n$ using lemmas @{thm[source] wf_E_bin} 
+and @{thm[source] wf_E_bin0}; lemma @{thm[source] wf_earley} follows by definition.
+\<close>
 
 section \<open>Soundness\<close>
 
 text\<open>
-TODO:
+Next, we proof the soundness of the generated items, or: $A \rightarrow \, \alpha \bullet \beta, i, j \in B \,\,\, \textrm{implies} \,\,\, A \, \xRightarrow{\ast} \, @{term \<omega>}[i..j) \beta$
+which is stated in terms of our formalization by the @{term sound_item} definition below. As mentioned previously, the general proof structure
+follows the proof for well-formedness. Thus, we only highlight one slightly more involved lemma stating the
+soundness of the @{term Complete} operation while stating the remaining lemmas without explicit proof.
+Additionally, proving lemma @{term sound_Complete} provides some insight into working with and proving properties
+about derivations.
 \<close>
 
 definition sound_item :: "'a cfg \<Rightarrow> 'a sentential \<Rightarrow> 'a item \<Rightarrow> bool" where
-  "sound_item cfg inp x = derives cfg [item_rule_head x] (slice (item_origin x) (item_end x) inp @ item_\<beta> x)"
+  "sound_item cfg \<omega> x = derives cfg [item_rule_head x] (slice (item_origin x) (item_end x) \<omega> @ item_\<beta> x)"
 
 definition sound_items :: "'a cfg \<Rightarrow> 'a sentential \<Rightarrow> 'a items \<Rightarrow> bool" where
-  "sound_items cfg inp I \<equiv> \<forall>x \<in> I. sound_item cfg inp x"
+  "sound_items cfg \<omega> I \<equiv> \<forall>x \<in> I. sound_item cfg \<omega> x"
 
-lemma sound_Init:
-  shows "sound_items cfg inp (Init cfg)"
+text\<open>
+Obua \cite{Obua:2017} \cite{LocalLexing-AFP} defines derivations at two different abstraction levels.
+The first representation is as the reflexive-transitive closure of the set of one-step derivations as introduced earlier in this chapter.
+The second representation is again more operational. He defines a predicate @{term "Derives1 cfg u i r v"}
+that is conceptually analogous to the predicate @{term "derives1 cfg u v"} but also captures the rule $r$
+used for a single rewriting step and the position $i$ in $u$ where the rewriting occurs.
+\<close>
+
+definition Derives1 :: "'a cfg \<Rightarrow> 'a sentential \<Rightarrow> nat \<Rightarrow> 'a rule \<Rightarrow> 'a sentential \<Rightarrow> bool" where
+  "Derives1 cfg u i r v \<equiv> 
+     \<exists> \<alpha> \<beta> N \<gamma>. 
+          u = \<alpha> @ [N] @ \<beta>
+        \<and> v = \<alpha> @ \<gamma> @ \<beta>
+        \<and> (N, \<gamma>) \<in> set (\<RR> cfg)
+        \<and> r = (N, \<gamma>) \<and> i = length \<alpha>"
+
+text\<open>
+We then define the type of a \textit{derivation} as a list of pairs representing precisely the positions and rules
+used to apply each rewrite step. The predicate @{term Derivation} is defined recursively as follows: $\alpha \Rightarrow \beta$ only
+holds for the empty derivation or list. If the derivation consists of at least one rewrite pair $(i, r)$, or
+@{term "Derivation cfg \<alpha> ((i, r)#D) \<beta>"}, then there must exist a $\gamma$ such that @{term "Derives1 cfg \<alpha> i r \<gamma>"} and
+@{term "Derivation cfg \<gamma> D \<beta>"}. Obua then proves that both notions of a derivation are equivalent (lemma @{term derives_equiv_Derivation})
+\<close>
+
+type_synonym 'a derivation = "(nat \<times> 'a rule) list"
+
+fun Derivation :: "'a cfg \<Rightarrow> 'a sentential \<Rightarrow> 'a derivation \<Rightarrow> 'a sentential \<Rightarrow> bool" where
+  "Derivation _ \<alpha> [] \<beta> = (\<alpha> = \<beta>)"
+| "Derivation cfg \<alpha> (d#D) \<beta> = (\<exists>\<gamma>. Derives1 cfg \<alpha> (fst d) (snd d) \<gamma> \<and> Derivation cfg \<gamma> D \<beta>)"
+
+lemma derives_equiv_Derivation:
+  shows "derives cfg \<alpha> \<beta> \<equiv> \<exists> D. Derivation cfg \<alpha> D \<beta>"
 (*<*)
   sorry
 (*>*)
 
-lemma sound_item_inc_item:
-  assumes "wf_item cfg inp x" "sound_item cfg inp x"
-  assumes "next_symbol x = Some a" "k < length inp" "inp!k = a" "item_end x = k"
-  shows "sound_item cfg inp (inc_item x (k+1))"
+text\<open>
+Next, we state a small but useful lemma about rewriting derivations using the more operational
+definition of derivations defined above without explicit proof.
+\<close>
+
+lemma Derivation_append_rewrite:
+  assumes "Derivation cfg \<alpha> D (\<beta> @ \<gamma> @ \<delta>) "
+  assumes "Derivation cfg \<gamma> E \<gamma>'"
+  shows "\<exists>F. Derivation cfg \<alpha> F (\<beta> @ \<gamma>' @ \<delta>)"
 (*<*)
   sorry
 (*>*)
 
-lemma sound_Scan:
-  assumes "wf_items cfg inp I" "sound_items cfg inp I"
-  shows "sound_items cfg inp (Scan k inp I)"
-(*<*)
-  sorry
-(*>*)
-
-lemma sound_Predict:
-  assumes "sound_items cfg inp I"
-  shows "sound_items cfg inp (Predict k cfg I)"
-(*<*)
-  sorry
-(*>*)
+text\<open>
+And finally, we proof soundness of the @{term Complete} operation:
+\<close>
 
 lemma sound_Complete:
-  assumes "wf_items cfg inp I" "sound_items cfg inp I"
-  shows "sound_items cfg inp (Complete k I)"
+  assumes wf: "wf_items cfg \<omega> I"
+  assumes sound: "sound_items cfg \<omega> I"
+  shows "sound_items cfg \<omega> (Complete k I)"
 (*<*)
   sorry
 (*>*)
+
+text\<open>
+\begin{proof}
+
+Let $z$ denote an arbitrary but fixed item of @{term "Complete k I"}. By the definition of the
+@{term Complete} operation there exist items $x$ and $y$ such that: @{term "x \<in> bin I (item_origin y)"},
+@{term "y \<in> bin I k"}, @{term "is_complete y"}, @{term "next_symbol x = Some (item_rule_head y)"}, and
+@{term "z = inc_item x k"}.
+
+Since $y$ is in bin $k$, it is complete and the set $I$ is sound (assumption \textit{sound}),
+there exists a derivation $E$ such that 
+  $$@{term "Derivation cfg [item_rule_head y] E (slice (item_origin y) (item_end y) \<omega>)"}$$
+by lemma @{thm[source] derives_equiv_Derivation}. Similarly, since $x$ is in bin @{term "item_origin y"} and due to assumption \textit{sound},
+there exists a derivation $D$ such that
+  $$ @{term "Derivation cfg [item_rule_head x] D (slice (item_origin x) (item_origin y) \<omega> @ item_\<beta> x)"}$$
+Note that @{term "item_\<beta> x = (item_rule_head y) # tl (item_\<beta> x)"} since the next symbol of $x$ is equal to
+the item rule head of $y$. Thus, by lemma @{thm[source] Derivation_append_rewrite}, and the definition of $D$ and $E$,
+there exists a derivation $F$ such that
+
+\begin{equation*}
+\begin{split}
+  & @{term "Derivation cfg [item_rule_head x] F (slice (item_origin x) (item_origin y) \<omega>)"} \, @ \\
+  & \quad \quad @{term "slice (item_origin y) (item_end y) \<omega> @ tl (item_\<beta> x)"}
+\end{split}
+\end{equation*}
+
+Additionally, we know that $x$ and $y$ are well-formed items due to the facts that $x$ is in bin @{term "item_origin y"},
+$y$ is in bin $k$, and the assumption @{term "wf_items cfg \<omega> I"}. Thus, we can discharge the assumptions of
+lemma @{thm[source] slice_append} (@{term "item_origin x \<le> item_origin y"} and @{term "item_origin y \<le> item_end y"})
+and have 
+  $$@{term "Derivation cfg [item_rule_head x] F (slice (item_origin x) (item_end y) \<omega> @ tl (item_\<beta> x))"}$$
+
+Moreover, since @{term "z = inc_item x k"} and the next symbol of x is the item rule head of y, it follows
+that @{term "tl (item_\<beta> x) = item_\<beta> z"}, and ultimately @{term "sound_item cfg \<omega> z"}, again by the definition
+of $z$ and lemma @{thm[source] derives_equiv_Derivation}.
+
+\end{proof}
+\<close>
+
+lemma sound_Init:
+  shows "sound_items cfg \<omega> (Init cfg)"
+(*<*)
+  sorry
+(*>*)
+
+text\<open>\<close>
+
+lemma sound_Scan:
+  assumes "wf_items cfg \<omega> I"
+  assumes "sound_items cfg \<omega> I"
+  shows "sound_items cfg \<omega> (Scan k \<omega> I)"
+(*<*)
+  sorry
+(*>*)
+
+text\<open>\<close>
+
+lemma sound_Predict:
+  assumes "sound_items cfg \<omega> I"
+  shows "sound_items cfg \<omega> (Predict k cfg I)"
+(*<*)
+  sorry
+(*>*)
+
+text\<open>\<close>
 
 lemma sound_E_step:
-  assumes "wf_items cfg inp I" "sound_items cfg inp I" 
-  shows "sound_items cfg inp (E_step k cfg inp I)"
+  assumes "wf_items cfg \<omega> I"
+  assumes "sound_items cfg \<omega> I" 
+  shows "sound_items cfg \<omega> (E_step k cfg \<omega> I)"
 (*<*)
   sorry
 (*>*)
+
+text\<open>\<close>
 
 lemma sound_funpower:
-  assumes "wf_items cfg inp I" "sound_items cfg inp I"
-  shows "sound_items cfg inp (funpower (E_step k cfg inp) n I)"
+  assumes "wf_items cfg \<omega> I"
+  assumes "sound_items cfg \<omega> I"
+  shows "sound_items cfg \<omega> (funpower (E_step k cfg \<omega>) n I)"
 (*<*)
   sorry
 (*>*)
+
+text\<open>\<close>
 
 lemma sound_E_bin:
-  assumes "wf_items cfg inp I" "sound_items cfg inp I"
-  shows "sound_items cfg inp (E_bin k cfg inp I)"
+  assumes "wf_items cfg \<omega> I"
+  assumes "sound_items cfg \<omega> I"
+  shows "sound_items cfg \<omega> (E_bin k cfg \<omega> I)"
 (*<*)
   sorry
 (*>*)
+
+text\<open>\<close>
 
 lemma sound_E_bin0:
-  shows "sound_items cfg inp (E_bin 0 cfg inp (Init cfg))"
+  shows "sound_items cfg \<omega> (E_bin 0 cfg \<omega> (Init cfg))"
 (*<*)
   sorry
 (*>*)
+
+text\<open>\<close>
 
 lemma sound_\<E>:
-  shows "sound_items cfg inp (\<E> k cfg inp)"
+  shows "sound_items cfg \<omega> (\<E> k cfg \<omega>)"
 (*<*)
   sorry
 (*>*)
+
+text\<open>\<close>
 
 lemma sound_earley:
-  shows "sound_items cfg inp (earley cfg inp)"
+  shows "sound_items cfg \<omega> (earley cfg \<omega>)"
 (*<*)
   sorry
 (*>*)
 
+text\<open>
+Finally, using @{thm[source] sound_earley} and the definitions of @{term sound_item}, @{term recognizing},
+@{term is_finished} and @{term is_complete} the final theorem follows: if the generated set of Earley
+items is @{term recognizing}, or contains a \textit{finished} item then there exists a derivation from
+the start symbol of the grammar to the input $\omega$.
+\<close>
+
 theorem soundness:
-  assumes "recognizing (earley cfg inp) cfg inp"
-  shows "derives cfg [\<SS> cfg] inp"
+  assumes "recognizing (earley cfg \<omega>) cfg \<omega>"
+  shows "derives cfg [\<SS> cfg] \<omega>"
 (*<*)
   sorry
 (*>*)
@@ -485,98 +627,141 @@ TODO:
 \<close>
 
 lemma Scan_\<E>:
-  assumes "i+1 \<le> k" "k \<le> length inp" "x \<in> bin (\<E> k cfg inp) i"
-  assumes "next_symbol x = Some a" "inp!i = a"
-  shows "inc_item x (i+1) \<in> \<E> k cfg inp"
+  assumes "i+1 \<le> k"
+  assumes "x \<in> bin (\<E> k cfg \<omega>) i"
+  assumes "next_symbol x = Some a"
+  assumes "k \<le> length \<omega>"
+  assumes "\<omega>!i = a"
+  shows "inc_item x (i+1) \<in> \<E> k cfg \<omega>"
 (*<*)
   sorry
 (*>*)
+
+text\<open>\<close>
 
 lemma Predict_\<E>:
-  assumes "i \<le> k" "x \<in> bin (\<E> k cfg inp) i" "next_symbol x = Some N" "(N,\<alpha>) \<in> set (\<RR> cfg)"
-  shows "init_item (N,\<alpha>) i \<in> \<E> k cfg inp"
+  assumes "i \<le> k"
+  assumes "x \<in> bin (\<E> k cfg \<omega>) i"
+  assumes "next_symbol x = Some N"
+  assumes "(N,\<alpha>) \<in> set (\<RR> cfg)"
+  shows "init_item (N,\<alpha>) i \<in> \<E> k cfg \<omega>"
 (*<*)
   sorry
 (*>*)
+
+text\<open>\<close>
 
 lemma Complete_\<E>:
-  assumes "i \<le> j" "j \<le> k" "x \<in> bin (\<E> k cfg inp) i" "next_symbol x = Some N" "(N,\<alpha>) \<in> set (\<RR> cfg)"
-  assumes "i = item_origin y" "y \<in> bin (\<E> k cfg inp) j" "item_rule y = (N,\<alpha>)" "is_complete y"
-  shows "inc_item x j \<in> \<E> k cfg inp"
+  assumes "i \<le> j"
+  assumes "j \<le> k"
+  assumes "x \<in> bin (\<E> k cfg \<omega>) i"
+  assumes "next_symbol x = Some N"
+  assumes "(N,\<alpha>) \<in> set (\<RR> cfg)"
+  assumes "y \<in> bin (\<E> k cfg \<omega>) j"
+  assumes "item_rule y = (N,\<alpha>)"
+  assumes "i = item_origin y"
+  assumes "is_complete y"
+  shows "inc_item x j \<in> \<E> k cfg \<omega>"
 (*<*)
   sorry
 (*>*)
 
-type_synonym 'a derivation = "(nat \<times> 'a rule) list"
-
-definition Derives1 :: "'a cfg \<Rightarrow> 'a sentential \<Rightarrow> nat \<Rightarrow> 'a rule \<Rightarrow> 'a sentential \<Rightarrow> bool" where
-  "Derives1 cfg u i r v \<equiv> 
-     \<exists> x y N \<alpha>. 
-          u = x @ [N] @ y
-        \<and> v = x @ \<alpha> @ y
-        \<and> (N, \<alpha>) \<in> set (\<RR> cfg)
-        \<and> r = (N, \<alpha>) \<and> i = length x"
-
-fun Derivation :: "'a cfg \<Rightarrow> 'a sentential \<Rightarrow> 'a derivation \<Rightarrow> 'a sentential \<Rightarrow> bool" where
-  "Derivation _ a [] b = (a = b)"
-| "Derivation cfg a (d#D) b = (\<exists> x. Derives1 cfg a (fst d) (snd d) x \<and> Derivation cfg x D b)"
+text\<open>\<close>
 
 definition partially_completed :: "nat \<Rightarrow> 'a cfg \<Rightarrow> 'a sentential \<Rightarrow> 'a items \<Rightarrow> ('a derivation \<Rightarrow> bool) \<Rightarrow> bool" where
-  "partially_completed k cfg inp I P \<equiv>
+  "partially_completed k cfg \<omega> I P \<equiv>
     \<forall>i j x a D.
-      i \<le> j \<and> j \<le> k \<and> k \<le> length inp \<and>
+      i \<le> j \<and> j \<le> k \<and> k \<le> length \<omega> \<and>
       x \<in> bin I i \<and> next_symbol x = Some a \<and>
-      Derivation cfg [a] D (slice i j inp) \<and> P D \<longrightarrow>
+      Derivation cfg [a] D (slice i j \<omega>) \<and> P D \<longrightarrow>
       inc_item x j \<in> I"
 
 lemma fully_completed:
-  assumes "j \<le> k" "k \<le> length inp"
-  assumes "x = Item (N,\<alpha>) d i j" "x \<in> I" "wf_items cfg inp I"
-  assumes "Derivation cfg (item_\<beta> x) D (slice j k inp)"
-  assumes "partially_completed k cfg inp I (\<lambda>D'. length D' \<le> length D)"
+  assumes "wf_items cfg \<omega> I"
+  assumes "j \<le> k" 
+  assumes "k \<le> length inp"
+  assumes "x = Item (N,\<alpha>) d i j"
+  assumes "x \<in> I"
+  assumes "Derivation cfg (item_\<beta> x) D (slice j k \<omega>)"
+  assumes "partially_completed k cfg \<omega> I (\<lambda>D'. length D' \<le> length D)"
   shows "Item (N,\<alpha>) (length \<alpha>) i k \<in> I"
 (*<*)
   sorry
 (*>*)
 
+text\<open>\<close>
+
 lemma partially_completed_\<E>:
   assumes "wf_cfg cfg"
-  shows "partially_completed k cfg inp (\<E> k cfg inp) (\<lambda>_. True)"
+  shows "partially_completed k cfg inp (\<E> k cfg \<omega>) (\<lambda>_. True)"
 (*<*)
   sorry
 (*>*)
+
+text\<open>\<close>
 
 lemma partially_completed_earley:
   assumes "wf_cfg cfg"
-  shows "partially_completed (length inp) cfg inp (earley cfg inp) (\<lambda>_. True)"
+  shows "partially_completed (length \<omega>) cfg \<omega> (earley cfg \<omega>) (\<lambda>_. True)"
 (*<*)
   sorry
 (*>*)
+
+text\<open>\<close>
+
+lemma Derivation_\<SS>1:
+  assumes "wf_cfg cfg"
+  assumes "is_sentence cfg \<omega>" 
+  assumes "Derivation cfg [\<SS> cfg] D \<omega>" 
+  shows "\<exists>\<alpha> E. Derivation cfg \<alpha> E \<omega> \<and> (\<SS> cfg,\<alpha>) \<in> set (\<RR> cfg)"
+(*<*)
+  sorry
+(*>*)
+
+text\<open>\<close>
 
 theorem completeness:
-  assumes "derives cfg [\<SS> cfg] inp" "is_sentence cfg inp" "wf_cfg cfg"
-  shows "recognizing (earley cfg inp) cfg inp"
+  assumes "wf_cfg cfg"
+  assumes "is_sentence cfg \<omega>"
+  assumes "derives cfg [\<SS> cfg] \<omega>"
+  shows "recognizing (earley cfg \<omega>) cfg \<omega>"
 (*<*)
   sorry
 (*>*)
 
-corollary
-  assumes "wf_cfg cfg" "is_sentence cfg inp"
-  shows "recognizing (earley cfg inp) cfg inp \<longleftrightarrow> derives cfg [\<SS> cfg] inp"
+text\<open>\<close>
+
+corollary correctness:
+  assumes "wf_cfg cfg"
+  assumes "is_sentence cfg \<omega>"
+  shows "recognizing (earley cfg inp) cfg \<omega> \<longleftrightarrow> derives cfg [\<SS> cfg] \<omega>"
 (*<*)
   sorry
 (*>*)
 
 section \<open>Finiteness\<close>
 
+text\<open>At last, we prove that the generated set of Earley items is finite. In Chapter \ref{chap:04}
+we are using this result to prove the termination of an executable version of the algorithm.
+
+Since @{term "earley cfg \<omega>"} only generates well-formed items (lemma @{thm[source] wf_earley}) it suffices
+to prove that there only exists a finite number of well-formed items. Define 
+  $$@{term "T = (set (\<RR> cfg) \<times> {0::nat..m} \<times> {0..length \<omega>} \<times> {0..length \<omega>}) "} $$
+where @{term "m = Max { length (rule_body r) | r. r \<in> set (\<RR> cfg) }"}. The set $T$ is finite and
+@{term "{ x | x. wf_item cfg \<omega> x }"} is a subset of mapping the @{term Item} constructor over $T$ (strictly speaking
+we need to first unpack the quadruple).
+\<close>
+
 lemma finiteness_UNIV_wf_item:
-  shows "finite { x | x. wf_item cfg inp x }"
+  shows "finite { x | x. wf_item cfg \<omega> x }"
 (*<*)
   sorry
 (*>*)
 
+text\<open>\<close>
+
 theorem finiteness:
-  shows "finite (earley cfg inp)"
+  shows "finite (earley cfg \<omega>)"
 (*<*)
   sorry
 (*>*)
